solvers/53.lean
@@ -1,3 +1,4 @@
+import ProjectEulerStatements.P53
 namespace ProjectEulerSolutions.P53
 
 partial def countCombinatoricSelections (limitN threshold : Nat) : Nat :=
@@ -20,11 +21,14 @@ partial def countCombinatoricSelections (limitN threshold : Nat) : Nat :=
 
 
 
-def solve (_n : Nat) :=
-  countCombinatoricSelections 100 1000000
+def solve (limitN threshold : Nat) :=
+  countCombinatoricSelections limitN threshold
+
+theorem equiv (limitN threshold : Nat) :
+    ProjectEulerStatements.P53.naive limitN threshold = solve limitN threshold := sorry
 
 end ProjectEulerSolutions.P53
 open ProjectEulerSolutions.P53
 
 def main : IO Unit := do
-  IO.println (solve 0)
+  IO.println (solve 100 1000000)
