solvers/58.lean
@@ -1,3 +1,4 @@
+import ProjectEulerStatements.P58
 namespace ProjectEulerSolutions.P58
 
 partial def powMod (a d n : Nat) : Nat :=
@@ -92,6 +93,9 @@ example : countDiagPrimes 7 = (8, 13) := by
 
 example : countDiagPrimes 5 = (5, 9) := by
   native_decide
+
+theorem equiv (ratioNum ratioDen : Nat) :
+    ProjectEulerStatements.P58.naive ratioNum ratioDen = solve ratioNum ratioDen := sorry
 
 end ProjectEulerSolutions.P58
 open ProjectEulerSolutions.P58
